src/Assembly/Syntax.v
@@ -207,8 +207,8 @@ Inductive OpCode :=
 | xchg
 | xor
 (* Vectorized opcodes *)
-| vaddps
-| vpaddq    (* Vector packed add quadword integers *)
+(* | vaddps
+| vpaddq    Vector packed add quadword integers *)
 | vmovq     (* Vector move quadword *)
 .
 
@@ -299,8 +299,8 @@ Definition accesssize_of_declaration (opc : OpCode) : option AccessSize :=
   | test
   | xchg
   | xor
-  | vaddps
-  | vpaddq
+  (* | vaddps
+  | vpaddq *)
   | vmovq
     => None
   end.
