src/Assembly/WithBedrock/Semantics.v
@@ -62,6 +62,8 @@ Definition get_reg (st : reg_state) (r : REG) : Z
   := let '(idx, shift, bitcount) := index_and_shift_and_bitcount_of_reg r in
   let rv := Tuple.nth_default 0%Z (N.to_nat idx) st in
   Z.land (Z.shiftr rv (Z.of_N shift)) (Z.ones (Z.of_N bitcount)).
+
+(* implicitly zeros the higher bits when v is smaller than bitcount.? *)
 Definition set_reg (st : reg_state) (r : REG) (v : Z) : reg_state
   := let '(idx, shift, bitcount) := index_and_shift_and_bitcount_of_reg r in
      Tuple.from_list_default 0%Z _ (ListUtil.update_nth
@@ -69,6 +71,7 @@ Definition set_reg (st : reg_state) (r : REG) (v : Z) : reg_state
        (fun curv => Z.lor (Z.shiftl (Z.land v (Z.ones (Z.of_N bitcount))) (Z.of_N shift))
                           (Z.ldiff curv (Z.shiftl (Z.ones (Z.of_N bitcount)) (Z.of_N shift))))
        (Tuple.to_list _ st)).
+
 Definition annotate_reg_state (st : reg_state) : list (REG * Z)
   := List.combine widest_registers (Tuple.to_list _ st).
 Ltac print_reg_state st := let st' := (eval cbv in (annotate_reg_state st)) in idtac st'.
@@ -111,7 +114,7 @@ Definition DenoteAddress (sa : N) (st : machine_state) (a : MEM) : Z :=
     match mem_scale_reg a with Some (z, r) => get_reg st r * DenoteConst sa z | _ => 0 end +
     match mem_offset    a with Some  z     =>                DenoteConst sa z | _ => 0 end
   ) (Z.ones (Z.of_N sa)).
-
+  
 Definition DenoteOperand (sa s : N) (st : machine_state) (a : ARG) : option Z :=
   match a with
   | reg a => Some (get_reg st a)
@@ -167,6 +170,10 @@ Definition DenoteNormalInstruction (st : machine_state) (instr : NormalInstructi
   | (mov | movzx | movabs | movdqa | movdqu | movq | movd | movups), [dst; src] => (* Note: unbundle when switching from N to Z *)
     v <- DenoteOperand sa s st src;
     SetOperand sa s st dst v
+  | vmovq, [dst; src] => (* move quadword - handles vector/scalar conversions *)
+    v <- DenoteOperand sa 64 st src;  (* Will still read a whole register.. *)
+    let v := Z.land v (Z.ones 64) in  (* Ensure 64-bit value *)
+    SetOperand sa 64 st dst v
   | xchg, [a; b] => (* Flags Affected: None *)
     va <- DenoteOperand sa s st a;
     vb <- DenoteOperand sa s st b;
@@ -216,85 +223,6 @@ Definition DenoteNormalInstruction (st : machine_state) (instr : NormalInstructi
     let v := Z.land v (Z.ones (Z.of_N s)) in
     st <- SetOperand sa s st dst v;
     Some (SetFlag st flag (Z.odd (Z.shiftr (v1 + v2 + c) (Z.of_N s))))
-  | vaddps, [dst; src1; src2] => (* single precision vector addition *)
-    let lane_size := 32%N in (* 8 32 bit floats *)
-    let extract_lane (v : Z) (lane_idx : N) : Z :=
-      Z.land (Z.shiftr v (Z.of_N (lane_size * lane_idx))) (Z.ones (Z.of_N lane_size)) in
-    v1_full <- DenoteOperand sa s st src1;
-    v2_full <- DenoteOperand sa s st src2;
-    let results := [
-      extract_lane v1_full 0%N + extract_lane v2_full 0%N;
-      extract_lane v1_full 1%N + extract_lane v2_full 1%N;
-      extract_lane v1_full 2%N + extract_lane v2_full 2%N;
-      extract_lane v1_full 3%N + extract_lane v2_full 3%N;
-      extract_lane v1_full 4%N + extract_lane v2_full 4%N;
-      extract_lane v1_full 5%N + extract_lane v2_full 5%N;
-      extract_lane v1_full 6%N + extract_lane v2_full 6%N;
-      extract_lane v1_full 7%N + extract_lane v2_full 7%N
-    ] in 
-    let v :=
-      Z.lor (Z.shiftl (nth_default 0 results 0) (Z.of_N (lane_size * 0)))
-      (Z.lor (Z.shiftl (nth_default 0 results 1) (Z.of_N (lane_size * 1)))
-      (Z.lor (Z.shiftl (nth_default 0 results 2) (Z.of_N (lane_size * 2)))
-      (Z.lor (Z.shiftl (nth_default 0 results 3) (Z.of_N (lane_size * 3)))
-      (Z.lor (Z.shiftl (nth_default 0 results 4) (Z.of_N (lane_size * 4)))
-      (Z.lor (Z.shiftl (nth_default 0 results 5) (Z.of_N (lane_size * 5)))
-      (Z.lor (Z.shiftl (nth_default 0 results 6) (Z.of_N (lane_size * 6)))
-      (Z.shiftl (nth_default 0 results 7) (Z.of_N (lane_size * 7)))
-      ))))))
-    in
-    st <- SetOperand sa s st dst v;
-    Some st
-  | vpaddq, [dst; src1; src2] => (* packed quadword integer addition *)
-    let lane_size := 64%N in (* 4 64-bit integers *)
-    let extract_lane (v : Z) (lane_idx : N) : Z :=
-      Z.land (Z.shiftr v (Z.of_N (lane_size * lane_idx))) (Z.ones (Z.of_N lane_size)) in
-    v1_full <- DenoteOperand sa s st src1;
-    v2_full <- DenoteOperand sa s st src2;
-    let results := [
-      Z.land (extract_lane v1_full 0%N + extract_lane v2_full 0%N) (Z.ones (Z.of_N lane_size));
-      Z.land (extract_lane v1_full 1%N + extract_lane v2_full 1%N) (Z.ones (Z.of_N lane_size));
-      Z.land (extract_lane v1_full 2%N + extract_lane v2_full 2%N) (Z.ones (Z.of_N lane_size));
-      Z.land (extract_lane v1_full 3%N + extract_lane v2_full 3%N) (Z.ones (Z.of_N lane_size))
-    ] in
-    let v :=
-      Z.lor (Z.shiftl (nth_default 0 results 0) (Z.of_N (lane_size * 0)))
-      (Z.lor (Z.shiftl (nth_default 0 results 1) (Z.of_N (lane_size * 1)))
-      (Z.lor (Z.shiftl (nth_default 0 results 2) (Z.of_N (lane_size * 2)))
-      (Z.shiftl (nth_default 0 results 3) (Z.of_N (lane_size * 3)))
-      ))
-    in
-    st <- SetOperand sa s st dst v;
-    Some st
-  | vmovq, [dst; src] => (* move quadword *)
-    (* vmovq handles several cases:
-       - vmovq xmm, r64: move 64-bit scalar to lower 64 bits of xmm, zero upper bits
-       - vmovq r64, xmm: move lower 64 bits of xmm to scalar register
-       - vmovq xmm, xmm/m64: move 64 bits, zero upper bits of destination
-       Note: Writing to XMM zeroes upper 128 bits of corresponding YMM (AVX convention) *)
-    match dst, src with
-    | reg (VReg dst_vr), reg (SReg src_sr) =>
-        (* vmovq xmm, r64 - move scalar to vector, zero upper bits *)
-        v <- DenoteOperand sa 64 st (SReg src_sr);
-        let v := Z.land v (Z.ones 64) in (* ensure 64-bit value *)
-        (* Only lower 64 bits set, rest is zero - this effectively zeros all upper bits *)
-        Some (update_reg_with st (fun rs => set_reg rs (VReg dst_vr) v))
-    | reg (SReg dst_sr), reg (VReg src_vr) =>
-        (* vmovq r64, xmm - extract lower 64 bits of vector to scalar *)
-        v_full <- DenoteOperand sa s st (VReg src_vr);
-        let v := Z.land v_full (Z.ones 64) in (* extract lower 64 bits *)
-        Some (update_reg_with st (fun rs => set_reg rs (SReg dst_sr) v))
-    | reg (VReg dst_vr), reg (VReg src_vr) =>
-        (* vmovq xmm, xmm - move lower 64 bits, zero upper bits of dst *)
-        v_full <- DenoteOperand sa s st (VReg src_vr);
-        let v := Z.land v_full (Z.ones 64) in (* extract lower 64 bits *)
-        Some (update_reg_with st (fun rs => set_reg rs (VReg dst_vr) v))
-    | _, _ =>
-        (* vmovq xmm, m64 or vmovq m64, xmm - use standard operand handling *)
-        v <- DenoteOperand sa 64 st src;
-        let v := Z.land v (Z.ones 64) in (* ensure 64-bit *)
-        SetOperand sa 64 st dst v
-    end
   | (sbb | sub) as opc, [dst; src] =>
     c <- (match opc with sbb => get_flag st CF | _ => Some false end);
     let c := Z.b2z c in
@@ -474,9 +402,6 @@ Definition DenoteNormalInstruction (st : machine_state) (instr : NormalInstructi
   | adox, _
   | and, _
   | bzhi, _
-  | vaddps, _
-  | vpaddq, _
-  | vmovq, _
   | db, _
   | dw, _
   | dd, _
@@ -498,6 +423,7 @@ Definition DenoteNormalInstruction (st : machine_state) (instr : NormalInstructi
   | lea, _
   | mov, _
   | movzx, _
+  | vmovq, _
   | or, _
   | imul, _
   | inc, _
